Model of the algorithm for universe checking inspired by Bezem et al
Terminating but incorrect loop check

Improved version, whose termination relies on the correctness of check_model

Move back to template-coq folder

Improve the algorithm after discussion with Marc Bezem

Comment a bit

Try enforcing new constraints

Reorganize inner loop

Cleaner inner_loop

Finished inner loop

Inner loop termination proven

Before change of v_minus_w_bound

Prove the well-foundedness of loop

Inner loop termination proof finished

Finished all proofs

Finish proofs of auxilliary lemmas

Finished all proofs with new invariants

Comments and extraction setup

Abstract LoopChecking on level / sets / maps implementation

Move clauses.v to LoopChecking and TemplateLoopChecking

Functorize the algorithm

Simplified loops

Cleaned up LoopChecking and TemplateLoopChecking

Support correct quoting/unquoting of the universe graph/context.
Also rename Constraint to LevelConstraint, preparing for a later move to general universe constraints

Add a new (extracted) plugin to test the loop checking algorithm.

Move back to subst_instance_cstr for level constraints

Move live tests of loop_checking to the test-suite

Revert changes to Universes.v

Avoid repeateadly folding over clauses in inner loop

Optimize a bit loop checking to avoid partitioning clause repeatedly

Fix UnivConstraint -> LevelConstraint change

Remove useless extraction file in template-coq

MSetList is no longer needed

template-rocq/src/ast_denoter.ml
@@ -27,7 +27,7 @@ struct
 
   type quoted_sort_family = Universes0.allowed_eliminations
   type quoted_constraint_type = Universes0.ConstraintType.t
-  type quoted_univ_constraint = Universes0.UnivConstraint.t
+  type quoted_univ_constraint = Universes0.LevelConstraint.t
   type quoted_univ_constraints = Universes0.ConstraintSet.t
   type quoted_univ_level = Universes0.Level.t
   type quoted_univ_instance = Universes0.Instance.t
