template-rocq/theories/TemplateMonad/Extractable.v
@@ -51,7 +51,7 @@ Cumulative Inductive TM@{t} : Type@{t} -> Type :=
   : TM mutual_inductive_body
 | tmQuoteConstant (nm : kername) (bypass_opacity : bool)
   : TM constant_body
-| tmQuoteUniverses : TM ConstraintSet.t
+| tmQuoteUniverses : TM ContextSet.t
 | tmQuoteModule : qualid -> TM (list global_reference)
 | tmQuoteModFunctor : qualid -> TM (list global_reference)
 | tmQuoteModType : qualid -> TM (list global_reference)
